refactor: P1.fst{,i} + P1_UInt32.fst + test.c

test.c
@@ -1,12 +1,12 @@
 #include "P1_UInt32.c"
 
 int main() {
-  uint32_t p = P1_UInt32_main ();
-  printf("r=%ui\n", p);
-  uint64_t h = P1_UInt32_main2 ();
-  printf("h=%lui\n", h);
-  uint64_t s = P1_UInt32_main3 ();
-  printf("s=%lui\n", s);
+  //uint32_t p = P1_UInt32_main ();
+  //printf("r=%ui\n", p);
+  //uint64_t h = P1_UInt32_main2 ();
+  //printf("h=%lui\n", h);
+  //uint64_t s = P1_UInt32_main3 ();
+  //printf("s=%lui\n", s);
   uint64_t r = P1_UInt32_main4 ();
   printf("r=%lui\n", r);
   return 0;
