P1_UInt32.fst
@@ -10,8 +10,8 @@ module I64 = FStar.Int64
 //open NTreeC3
 //open P1
 
-let t = NTreeC3.t
-let linked_tree = NTreeC3.linked_tree
+let t = Impl.Core.t
+let linked_tree = Impl.Core.linked_tree
 
 //let a = U32.t
 //let val0 = 0ul
@@ -42,45 +42,45 @@ let compare (x y: a) : I64.t
   else -1L
 
 inline_for_extraction noextract
-let get_left = NTreeC3.get_left #a
+let get_left = Impl.Core.get_left #a
 inline_for_extraction noextract
-let get_right = NTreeC3.get_right #a
+let get_right = Impl.Core.get_right #a
 inline_for_extraction noextract
-let get_size = NTreeC3.get_size #a
+let get_size = Impl.Core.get_size #a
 inline_for_extraction noextract
-let get_data = NTreeC3.get_data #a
+let get_data = Impl.Core.get_data #a
 
 // will be useful later? if so, null or null_t?
 //inline_for_extraction noextract
 //let null = Steel.Reference.null
 inline_for_extraction noextract
-let is_null_t = NTreeC3.is_null_t #a
+let is_null_t = Impl.Core.is_null_t #a
 
 inline_for_extraction noextract
-let mk_node = NTreeC3.mk_node #a
+let mk_node = Impl.Core.mk_node #a
 
 (* not inlined *)
-let unpack_tree = NTreeC3.unpack_tree #a
+let unpack_tree = Impl.Core.unpack_tree #a
 
 (* stdlib *)
-let create_leaf = P1.create_leaf #a
-let create_tree = P1.create_tree #a
-let merge_tree = P1.merge_tree #a
-let sot_wds = P1.sot_wds #a
-let append_left = P1.append_left #a
-let append_right = P1.append_right #a
-let height = P1.height #a
-let member = P1.member #a
-let insert_bst = P1.insert_bst #a
-let insert_bst2 = P1.insert_bst2 #a
-let rotate_left = P1.rotate_left #a
-let rotate_right = P1.rotate_right #a
-let rotate_right_left = P1.rotate_right_left #a
-let rotate_left_right = P1.rotate_left_right #a
-let is_balanced = P1.is_balanced #a
-let rebalance_avl = P1.rebalance_avl #a
-let insert_avl = P1.insert_avl #a
-let insert_avl2 = P1.insert_avl2 #a
+//let append_left = P1.append_left #a
+//let append_right = P1.append_right #a
+//let insert_bst = P1.insert_bst #a
+//let insert_avl = Impl.insert_avl #a
+let create_leaf = Impl.create_leaf #a
+let create_tree = Impl.create_tree #a
+let merge_tree  = Impl.merge_tree #a
+let sot_wds     = Impl.sot_wds #a
+let heighti     = Impl.height #a
+let member      = Impl.member #a
+//let insert_bst2 = Impl.insert_bst2 #a
+let rotate_left = Impl.rotate_left #a
+let rotate_right = Impl.rotate_right #a
+let rotate_right_left = Impl.rotate_right_left #a
+let rotate_left_right = Impl.rotate_left_right #a
+let is_balanced = Impl.is_balanced #a
+let rebalance_avl = Impl.rebalance_avl #a
+let insert_avl2 = Impl.insert_avl2 #a
 
 (*
 let one ()
@@ -119,34 +119,34 @@ let rec destruct (ptr: t a) : Steel unit
   )*)
 
 
-let main ()
-  : Steel U32.t
-  (emp)
-  (fun _ -> emp)
-  (requires fun _ -> True)
-  (ensures fun _ _ _-> True)
-  =
-  let ptr = create_tree val1 in
-  let ptr = append_left ptr val2 in
-  let b = member ptr val1 in
-  let vr = if b then val42 else val0 in
-  destruct ptr;
-  return (fst vr)
+//let main ()
+//  : Steel U32.t
+//  (emp)
+//  (fun _ -> emp)
+//  (requires fun _ -> True)
+//  (ensures fun _ _ _-> True)
+//  =
+//  let ptr = create_tree val1 in
+//  let ptr = append_left ptr val2 in
+//  let b = member ptr val1 in
+//  let vr = if b then val42 else val0 in
+//  destruct ptr;
+//  return (fst vr)
 
-let main2 ()
-  : Steel U64.t
-  (emp)
-  (fun n -> emp)
-  (requires fun _ -> True)
-  (ensures fun _ _ _-> True)
-  =
-  let ptr = create_leaf () in
-  let ptr = append_right ptr val1 in
-  let ptr = append_right ptr val2 in
-  let ptr = append_right ptr val3 in
-  let h = height ptr in
-  destruct ptr;
-  h
+//let main2 ()
+//  : Steel U64.t
+//  (emp)
+//  (fun n -> emp)
+//  (requires fun _ -> True)
+//  (ensures fun _ _ _-> True)
+//  =
+//  let ptr = create_leaf () in
+//  let ptr = append_right ptr val1 in
+//  let ptr = append_right ptr val2 in
+//  let ptr = append_right ptr val3 in
+//  let h = height ptr in
+//  destruct ptr;
+//  h
 
 
 let compare_is_cmp () : Lemma
@@ -157,30 +157,29 @@ let compare_is_cmp () : Lemma
   (forall x  y z. I64.gte (compare x y) I64.zero /\
                          I64.gte (compare y z) I64.zero ==>
                          I64.gte (compare x z) I64.zero)
-) = admit ()
+) = ()
 
-#set-options "--z3rlimit 50"
-let main3 ()
-  : Steel U32.t
-  emp (fun r_n -> emp)
-  (requires fun _ -> True)
-  (ensures fun _ _ _-> True)
-  =
-  let ptr = create_leaf () in
-  let ptr = append_left ptr val0 in
-  let ptr = append_right ptr val1 in
-  let ptr = insert_avl compare ptr val3 in
-  //let h = get () in
-  //compare_is_cmp ();
-  //assert (Trees.is_bst (P1.convert compare) (NTreeC3.v_linked_tree ptr h));
-  let ptr = insert_bst compare ptr val2 in
-  //let h = get () in
-  //assert (Trees.is_bst (P1.convert compare) (NTreeC3.v_linked_tree ptr h));
-  let h = sot_wds ptr in
-  let b = member ptr val3 in
-  let vr = if b then val42 else val0 in
-  destruct ptr;
-  return (fst vr)
+//let main3 ()
+//  : Steel U32.t
+//  emp (fun r_n -> emp)
+//  (requires fun _ -> True)
+//  (ensures fun _ _ _-> True)
+//  =
+//  let ptr = create_leaf () in
+//  let ptr = append_left ptr val0 in
+//  let ptr = append_right ptr val1 in
+//  let ptr = insert_avl compare ptr val3 in
+//  //let h = get () in
+//  //compare_is_cmp ();
+//  //assert (Trees.is_bst (P1.convert compare) (NTreeC3.v_linked_tree ptr h));
+//  let ptr = insert_bst compare ptr val2 in
+//  //let h = get () in
+//  //assert (Trees.is_bst (P1.convert compare) (NTreeC3.v_linked_tree ptr h));
+//  let h = sot_wds ptr in
+//  let b = member ptr val3 in
+//  let vr = if b then val42 else val0 in
+//  destruct ptr;
+//  return (fst vr)
 
 let main4()
   : Steel U32.t
@@ -197,7 +196,7 @@ let main4()
   let ptr = insert_avl2 f compare ptr valn1 in
   let ptr = insert_avl2 f compare ptr valn2 in
   assert (I64.eq (compare valn1 valn2) I64.zero);
-  let b = member ptr valn2 in
+  let b = member compare ptr valn2 in
   let vr = if b then val42 else val0 in
   destruct ptr;
   return (fst vr)
